AP/Temp.lean
@@ -16,6 +16,8 @@ end Nat
 
 namespace Int
 
+attribute [simp] not_ofNat_neg
+
 -- #check 0 #exit
 
 end Int
